RepairSpill: switched to pick_kill/pick_load

theories/Spilling/PickLK.v
@@ -3,32 +3,32 @@ Require Import Take TakeSet.
 
 Set Implicit Arguments.
 
-(* pick_kill' *)
+(* pick *)
 
-Definition pick_kill' (X:Type) `{OrderedType X} (k : nat) (s t : ⦃X⦄) : ⦃X⦄
+Definition pick (X:Type) `{OrderedType X} (k : nat) (s t : ⦃X⦄) : ⦃X⦄
   := s ∪ set_take (k - cardinal s) (t \ s)
 .
 
-Lemma incl_pick_kill' (X:Type) `{OrderedType X} (k : nat) (s t : ⦃X⦄) :
-  s ⊆ pick_kill' k s t
+Lemma incl_pick (X:Type) `{OrderedType X} (k : nat) (s t : ⦃X⦄) :
+  s ⊆ pick k s t
 .
 Proof.
-  unfold pick_kill'. cset_tac.
+  unfold pick. cset_tac.
 Qed.
 
-Lemma pick_kill'_incl (X:Type) `{OrderedType X} (k : nat) (s t : ⦃X⦄) :
-  pick_kill' k s t ⊆ s ∪ t
+Lemma pick_incl (X:Type) `{OrderedType X} (k : nat) (s t : ⦃X⦄) :
+  pick k s t ⊆ s ∪ t
 .
 Proof.
-  unfold pick_kill'. rewrite set_take_incl. cset_tac.
+  unfold pick. rewrite set_take_incl. cset_tac.
 Qed.
 
-Lemma pick_kill'_card (X:Type) `{OrderedType X} (k : nat) (s t : ⦃X⦄) :
+Lemma pick_card (X:Type) `{OrderedType X} (k : nat) (s t : ⦃X⦄) :
   k <= cardinal (s ∪ t)
-  -> k <= cardinal (pick_kill' k s t)
+  -> k <= cardinal (pick k s t)
 .
 Proof.
-  intros card. unfold pick_kill'. rewrite union_cardinal.
+  intros card. unfold pick. rewrite union_cardinal.
   - unfold set_take. rewrite cardinal_of_list_nodup; [|apply take_dupFree].
     assert (s ∪ t [=] s ∪ t \ s) as seteq by cset_tac.
     rewrite seteq in card. rewrite union_cardinal in card; [|clear;cset_tac].
@@ -38,26 +38,54 @@ Proof.
   - intros. rewrite set_take_incl. cset_tac.
 Qed.
 
+Lemma pick_card' (X:Type) `{OrderedType X} (k : nat) (s t : ⦃X⦄) :
+  cardinal s <= k -> cardinal (pick k s t) <= k
+.
+Proof.
+  intros card. unfold pick. rewrite union_cardinal.
+  - unfold set_take.  rewrite cardinal_of_list_nodup; [|apply take_dupFree].
+    decide (k - cardinal s <= cardinal (t \ s)).
+    + rewrite take_length_le; eauto.
+      * omega.
+      * rewrite elements_length. eauto.
+    + rewrite take_length_ge; eauto.
+      * rewrite elements_length. omega.
+      * rewrite elements_length. omega.
+  - intros. rewrite set_take_incl. cset_tac.
+Qed.
+  
+
+Lemma pick_eq (X:Type) `{OrderedType X} k (s t : ⦃X⦄)
+  : cardinal s + cardinal (t \ s) <= k -> pick k s t [=] s ∪ t
+.
+Proof.
+  intros card. apply incl_eq; [|apply pick_incl].
+  unfold pick. unfold set_take.
+  rewrite take_eq_ge.
+  - rewrite of_list_elements. cset_tac.
+  - rewrite elements_length. unfold ">=". apply Nat.le_add_le_sub_r.
+    omega.
+Qed.
 
 (* pick_kill *)
              
 Definition pick_kill (X:Type) `{OrderedType X} (k:nat) (s t u v : ⦃X⦄) : ⦃X⦄
-  := pick_kill' (cardinal s + cardinal t - k) ((s \ (u ∪ v)) ∪ (s ∩ t)) (s ∩ v \ u)
+  := pick (cardinal s + cardinal t - k) ((s \ (u ∪ v)) ∪ (s ∩ t)) (s ∩ v \ u)
 .
 
 Lemma incl_pick_kill (X:Type) `{OrderedType X} (k:nat) (s t u v : ⦃X⦄) :
   ((s \ (u ∪ v)) ∪ (s ∩ t)) ⊆ pick_kill k s t u v
 .
 Proof.
-  eapply incl_pick_kill'.
+  eapply incl_pick.
 Qed.
 
 
 Lemma pick_kill_incl (X:Type) `{OrderedType X} (k : nat) (s t u v : ⦃X⦄) :
-  pick_kill k s t u v ⊆ (s ∪ v) \ u ∪ (s ∩ t)
+  pick_kill k s t u v ⊆ (s ∩ t) ∪ (s \ u)
 .
 Proof.
-  unfold pick_kill. rewrite pick_kill'_incl. cset_tac.
+  unfold pick_kill. rewrite pick_incl. cset_tac.
 Qed.
 
 Lemma pick_kill_card (X:Type) `{OrderedType X} (k : nat) (s t u v : ⦃X⦄) :
@@ -68,28 +96,97 @@ Proof.
   intros card.
   assert (s ∩ u \ t [=] s \ (((s \ (u ∪ v)) ∪ (s ∩ t)) ∪ (s ∩ v \ u))) as seteq by cset_tac.
   rewrite seteq in card. rewrite cardinal_difference' in card; [|clear;cset_tac].
-  eapply pick_kill'_card. omega.
+  eapply pick_card. omega.
 Qed.
   
 (* pick_killx *)
 
 Definition pick_killx (X:Type) `{OrderedType X} (k:nat) (x:X) (s t : ⦃X⦄) : ⦃X⦄
-  := pick_kill' (cardinal {x; s} - k) (s \ t) (s ∩ t)
+  := pick (cardinal {x; s} - k) (s \ t) (s ∩ t)
 .
 
 Lemma incl_pick_killx (X:Type) `{OrderedType X} (k:nat) (x:X) (s t : ⦃X⦄) :
   s \ t ⊆ pick_killx k x s t
 .
 Proof.
-  eapply incl_pick_kill'.
+  eapply incl_pick.
 Qed.
 
 Lemma pick_killx_incl (X:Type) `{OrderedType X} (k:nat) (x:X) (s t : ⦃X⦄) :
   pick_killx k x s t ⊆ s
 .
 Proof.
-  unfold pick_killx. rewrite pick_kill'_incl. clear;cset_tac.
+  unfold pick_killx. rewrite pick_incl. clear;cset_tac.
 Qed.
 
 
+(* pick_load *)
 
+Definition pick_load (X:Type) `{OrderedType X} (k:nat)  (r m sp l fv : ⦃X⦄) : ⦃X⦄ 
+  := pick (k - cardinal (fv ∩ r \ (l ∩ (sp ∪ m)))) (fv \ r) (l ∩ (sp ∩ r ∪ m))
+.
+
+
+Lemma incl_pick_load (X:Type) `{OrderedType X} (k:nat)  (r m sp l fv : ⦃X⦄) :
+  fv \ r ⊆ pick_load k r m sp l fv
+.
+Proof.
+  eapply incl_pick.
+Qed.
+(*
+Lemma incl_pick_load' (X:Type) `{OrderedType X} (k:nat)  (r m sp l fv : ⦃X⦄) :
+  cardinal fv -> fv \ r ⊆ pick_load k r m sp l fv
+.
+*)
+
+Lemma pick_load_eq (X:Type) `{OrderedType X} (k:nat)  (r m sp l fv : ⦃X⦄) :
+  sp ⊆ r
+  -> l ⊆ sp ∪ m
+  -> fv \ r ⊆ l
+  -> cardinal (fv ∪ l) <= k
+  -> pick_load k r m sp l fv [=] l
+.
+Proof.
+  intros spr lspm fvrl card.
+  assert (sp ∩ r [=] sp) as speq by (apply inter_subset_equal; eauto).
+  assert (l ∩ (sp ∩ r ∪ m) [=] l) as leq
+      by (apply inter_subset_equal in lspm; rewrite speq, lspm; eauto).
+  unfold pick_load.
+  rewrite pick_eq.
+  - rewrite leq. clear - fvrl. cset_tac.
+  - rewrite leq. rewrite <-union_cardinal.
+    + apply Nat.le_add_le_sub_r.
+      setoid_rewrite inter_subset_equal at 2;eauto.
+      rewrite <-union_cardinal.
+      * rewrite subset_cardinal; eauto. clear; cset_tac.
+      * clear. intros. intro N. cset_tac.
+    + clear. intros. intro N. cset_tac.
+Qed.
+      
+     
+
+(*
+Lemma pick_load_card (X:Type) `{OrderedType X} (k:nat) (r m sp l fv : ⦃X⦄) :
+  cardinal (pick_load k r m sp l fv) <= k
+.
+                                                                              
+  *)         
+
+
+Lemma pick_load_incl (X:Type) `{OrderedType X} (k:nat) (r m sp l fv : ⦃X⦄) :
+  pick_load k r m sp l fv ⊆ (sp ∩ r) ∪ m ∪ (fv \ r)
+.
+Proof.
+  unfold pick_load. rewrite pick_incl. cset_tac.
+Qed.
+
+Lemma pick_load_card (X:Type) `{OrderedType X} (k:nat) (r m sp l fv : ⦃X⦄) :
+  cardinal fv <= k -> cardinal (pick_load k r m sp l fv) <= k - cardinal (fv ∩ r \ (l ∩ (sp ∪ m)))
+.
+Proof.
+  intros card. unfold pick_load. rewrite pick_card'; eauto.
+  - apply Nat.le_add_le_sub_r. rewrite <-union_cardinal; [|clear;intros;cset_tac].
+    rewrite subset_cardinal; eauto. clear; cset_tac.
+Qed.
+
+  
