theories/Spilling/RepairSpill.v
@@ -35,7 +35,7 @@ Fixpoint repair_spill
 
   | stmtLet x e s, ann1 _ rlv', ann1 _ lv', ann1 (Sp,L,_) sl'
     => let Fv_e := Exp.freeVars e in (* this v has to be done also elsewhere !!!! *)
-      let L'   := set_take_prefer (k - cardinal (Fv_e ∩ R \ L)) (L ∩ ((Sp ∩ R) ∪ M)) (Fv_e \ R) in
+      let L'   := pick_load k R M Sp L Fv_e in
       (* we only use register liveness at 3 points to make some preferences
          in the selection of the kill set: (here)
          if the register liveness is incorrect we will still get a correct spilling *)
@@ -48,13 +48,13 @@ Fixpoint repair_spill
            
   | stmtReturn e, _, _, ann0 (Sp,L,_)
     => let Fv_e := Op.freeVars e in
-      let L'   := set_take_prefer (k - cardinal (Fv_e ∩ R \ L)) (L ∩ ((Sp ∩ R) ∪ M)) (Fv_e \ R) in
+      let L'   := pick_load k R M Sp L Fv_e in
       let Sp'  := Sp ∩ R in
       ann0 (Sp',L',nil)
 
   | stmtIf e s1 s2, ann2 _ rlv1 rlv2, ann2 _ lv1 lv2, ann2 (Sp,L,_) sl1 sl2
     => let Fv_e := Op.freeVars e in
-      let L'   := set_take_prefer (k - cardinal (Fv_e ∩ R \ L)) (L ∩ ((Sp ∩ R) ∪ M)) (Fv_e \ R) in
+      let L'   := pick_load k R M Sp L Fv_e in
       (* here is the second use of register liveness *)
       let K    := pick_kill k R L' (Op.freeVars e) (getAnn rlv1 ∪ getAnn rlv2) in
       let Sp'  := ((getAnn lv1 ∪ getAnn lv2) ∩ K \ M) ∪ (Sp ∩ R) in
@@ -67,7 +67,7 @@ Fixpoint repair_spill
       let R_f := fst (nth (counted f) Λ (∅,∅)) in
       let M_f := snd (nth (counted f) Λ (∅,∅)) in
       let Z   := nth (counted f) ZL nil in
-      let L'  := set_take_prefer k (L ∩ ((Sp ∩ R) ∪ M)) (R_f \ of_list Z \ R) in
+      let L'  := pick_load k R M Sp L (R_f \ of_list Z) in
       let K   := pick_kill k R L' (R_f \ of_list Z) (list_union (Op.freeVars ⊝ Y) \ M') in
       let M'' := (M \ (R \ K ∪ L)) ∩ fv_Y ∪ (M' ∩ (Sp ∪ M)) in
       let Sp' := ((fv_Y ∩ K \ M) ∪ (M_f  \ of_list Z \ M)) ∪ (Sp ∩ R) in
@@ -77,7 +77,7 @@ Fixpoint repair_spill
     => let rms' := stretch_rms k F rms (getAnn ⊝ lv_F) in
       let ZL'  := fst ⊝ F ++ ZL in
       let Λ'   := rms' ++ Λ in
-      let L'   := set_take k (L ∩ ((Sp ∩ R) ∪ M)) in
+      let L'   := pick_load k R M Sp L ∅ in
       (* here is the third use of register liveness *)
       let K    := pick_kill k R L' ∅ (getAnn rlv_t) in
       let Sp'  := ((getAnn lv_t) ∩ K \ M) ∪ (Sp ∩ R) in
