theories/Spilling/RepairSpillSound.v
@@ -1,7 +1,7 @@
 Require Import RepairSpill RegLive ExpVarsBounded.
 Require Import SpillSound Annotation Liveness.Liveness RenamedApart.
 Require Import List Map IL.
-Require Import Take TakeSet PickLK.
+Require Import Take TakeSet PickLK SetUtil.
 
 Set Implicit Arguments.
 
@@ -38,20 +38,18 @@ Proof.
   intros lvSnd anno_sl anno_rlv lv_RM expB (*rena RM_ra*).
   general induction lvSnd; invc anno_sl; invc anno_rlv; invc expB; (*invc rena;*) cbn.
   - destruct a,p. rename s0 into Sp. rename s1 into L. rename a0 into Rlv.
-    set (L' := set_take_prefer (k - cardinal (Exp.freeVars e ∩ R \ L))
-                               (L ∩ (Sp ∩ R ∪ M)) (Exp.freeVars e \ R)) in *.
+    set (L' := pick_load k R M Sp L (Exp.freeVars e)) in *.
     set (K' := pick_kill k R L' (Exp.freeVars e) Rlv) in *.
     set (Kx' := pick_killx k x (R \ K' ∪ L') Rlv) in *.
     set (Sp':= (getAnn al ∩ (K' ∪ Kx') \ M ∪ (Sp ∩ R))) in *.
     assert (Sp ∩ R ⊆ Sp') as Spincl.
     { subst Sp'. clear; cset_tac. }
-    econstructor; eauto.
-    + subst Sp'. apply incl_minus_incl_union in H0. rewrite H0.
-      subst Kx'. rewrite pick_killx_incl. subst K'.
-      setoid_rewrite pick_kill_incl at 1.
-      subst L'. setoid_rewrite set_take_prefer_incl at 1.
-      clear; cset_tac.
-    + subst L'. rewrite set_take_prefer_incl. rewrite Spincl.
+    econstructor; eauto; cbn in *.
+    + subst Sp'. subst K'. rewrite pick_kill_incl. setoid_rewrite meet_in_left at 2.
+      subst Kx'. rewrite pick_killx_incl.
+      setoid_rewrite minus_incl at 2 3. subst L'. rewrite pick_load_incl.
+      apply Exp.freeVars_live in H. rewrite H. rewrite lv_RM. clear; cset_tac.
+    + subst L'. rewrite pick_load_incl. rewrite <-Spincl.
       cbn in *. apply Exp.freeVars_live in H. rewrite H. clear - lv_RM. cset_tac.
     + eapply IHlvSnd; eauto. apply incl_minus_incl_union in H0.
       setoid_rewrite <-inter_subset_equal with (s':=getAnn al) at 1; eauto.
@@ -62,43 +60,27 @@ Proof.
       setoid_rewrite set_decomp with (t:=(K' ∪ Kx')) at 1.
       apply union_incl_split; [|cset_tac]. setoid_rewrite <-incl_right at 2.
       setoid_rewrite set_decomp with (t:=M) at 1; cset_tac.
-    + subst L'. cbn in *. 
-      subst K'. rewrite set_take_least_avoid_incl. admit. (*rewrite <-set_take_prefer_card_incl.
-      * rewrite <-minus_union. clear; cset_tac.
-      * apply Nat.le_add_le_sub_l. rewrite <-union_cardinal; [|clear;cset_tac].
-        rewrite <-set_decomp. eauto. *)
+    + subst K'. rewrite pick_kill_incl.
+      setoid_rewrite union_comm at 2. rewrite <-minus_union, minus_minus.
+      rewrite incl_minus_union; [|clear;cset_tac].
+      subst L'. rewrite <-incl_pick_load. clear; cset_tac.
     + assert (K' ⊆ R) as KReq.
-      { subst K'. rewrite set_take_least_avoid_incl. clear; cset_tac. }
+      { subst K'. rewrite pick_kill_incl. clear; cset_tac. }
       assert (disj (R \ K') L') as RKLdisj.
-      { subst K' L'.
-      setoid_rewrite set_decomp with (t:=R) at 5. rewrite <-union_assoc.
-      rewrite union_cardinal; [|clear;cset_tac].
-      setoid_rewrite cardinal_difference'.
-      setoid_rewrite set_take_least_avoid_size at 2; eauto.  
-      rewrite cardinal_union_split.
-      assert (forall s t u : ⦃var⦄, s \ t ∩ u [=] (s ∩ u) \ t) as seteq by (clear;intros;cset_tac).
-      rewrite seteq. setoid_rewrite cardinal_difference' at 2.
-
-      
-                                                                     
-                                                                     
-      subst K'. rewrite minus_union, minus_minus.
-      rewrite meet_in_left. rewrite union_cardinal_inter. subst L'.
-      apply <-Nat.le_sub_le_add_r. setoid_rewrite set_take_prefer_size at 1.
-      assert (cardinal R <= k) as cheat by admit.
-      rewrite cheat.
-      enough ((k - cardinal (Exp.freeVars e ∩ R))
-                             <= cardinal
-                                 (R ∩ set_take_prefer (k - cardinal (Exp.freeVars e ∩ R))
-                                    (L ∩ (Sp ∩ R ∪ M)) (Exp.freeVars e \ R))) by omega.
-      rewrite Nat.le_sub_le_add_r.
-      rewrite <-set_take_prefer_card_incl.
-      * 
-      setoid_rewrite set_take_prefer_incl at 2.
-      cset_tac.
-      subst Kx'. rewrite set_take_least_avoid_incl. subst K'. rewrite set_take_least_avoid_incl.
-      cbn in *. subst Sp'. setoid_rewrite set_take_least_avoid_incl at 1.
-      subst L'. setoid_rewrite set_take_prefer_incl at 1.
-  
+      { subst K'. rewrite <-incl_pick_kill. clear. cset_tac. }
+      rewrite union_cardinal; [|clear - RKLdisj;intros;intro N;cset_tac].
+      rewrite cardinal_difference'; eauto.
+      rewrite <-Nat.add_sub_swap; [|rewrite subset_cardinal; eauto].
+      apply Nat.le_sub_le_add_r.
+      subst K'. rewrite <-pick_kill_card; [omega|].
+      subst L'. rewrite pick_load_card; eauto.
+      assert (forall n1 n2 n3 : nat, n1 <= n3 -> n3 <= n2 -> n1 + (n2 - n3) <= n2) as nateq.
+      { clear. intros. omega. }
+      apply nateq; eauto.
+      * apply subset_cardinal;eauto. rewrite <-incl_pick_load; eauto.
+        admit. (*rewrite <-incl_pick_load. clear; cset_tac.*)
+      * rewrite subset_cardinal; eauto. clear; cset_tac.
+    + 
+  - 
   
                 
